@prefix dct: <http://purl.org/dc/terms/> .
@prefix foaf: <http://xmlns.com/foaf/0.1/> .
@prefix ical: <http://www.w3.org/2002/12/cal/icaltzd#> .
@prefix ns1: <http://dbpedia.org/ontology/> .
@prefix owl: <http://www.w3.org/2002/07/owl#> .
@prefix prv: <http://purl.org/net/provenance/ns#> .
@prefix rdfs: <http://www.w3.org/2000/01/rdf-schema#> .
@prefix teach: <http://linkedscience.org/teach/ns#> .
@prefix xhv: <http://www.w3.org/1999/xhtml/vocab#> .
@prefix xsd: <http://www.w3.org/2001/XMLSchema#> .

<http://http://ifgi.uni-muenster.de/~j_tram02/foaf.rdf> a foaf:Person;
    foaf:homepage <http://ifgi.uni-muenster.de/~j_tram02/>,
        <http://www.xing.com/profile/Andres_Westermann>;
    foaf:name "Andres Westermann"@en,
        "Johannes Trame"@en .

teach:Assignment a owl:Class;
    rdfs:label "Assignment"@en;
    rdfs:comment """Assignment of a course, for example an exercise.
"""@en;
    rdfs:isDefinedBy <http://linkedscience.org/teach/ns> .

teach:Building a owl:Class;
    rdfs:label "Building"@en;
    rdfs:comment """Building where the course is taking place.
"""@en;
    rdfs:isDefinedBy <http://linkedscience.org/teach/ns> .

teach:Course a owl:Class;
    rdfs:label "Course"@en;
    rdfs:comment """Course is where students are supposed to learn something.
"""@en;
    rdfs:isDefinedBy <http://linkedscience.org/teach/ns> .

teach:Lecture a owl:Class;
    rdfs:label "Lecture"@en;
    rdfs:comment """Lecture of the course.
"""@en;
    rdfs:isDefinedBy <http://linkedscience.org/teach/ns> .

teach:Material a owl:Class;
    rdfs:label "Material"@en;
    rdfs:comment """Material of the course.
"""@en;
    rdfs:isDefinedBy <http://linkedscience.org/teach/ns> .

teach:Module a owl:Class;
    rdfs:label "Module"@en;
    rdfs:comment """Module (i.e. a set of courses) which the course belongs to.
"""@en;
    rdfs:isDefinedBy <http://linkedscience.org/teach/ns> .

teach:Room a owl:Class;
    rdfs:label "Room"@en;
    rdfs:comment """Room where the course is taking place.
"""@en;
    rdfs:isDefinedBy <http://linkedscience.org/teach/ns> .

teach:Student a owl:Class;
    rdfs:label "Student"@en;
    rdfs:comment """Student of the course.
"""@en;
    rdfs:isDefinedBy <http://linkedscience.org/teach/ns> .

teach:StudentGroup a owl:Class;
    rdfs:label "StudentGroup"@en;
    rdfs:comment """StudentGroup of the course.
"""@en;
    rdfs:isDefinedBy <http://linkedscience.org/teach/ns> .

teach:StudyProgram a owl:Class;
    rdfs:label "StudyProgram"@en;
    rdfs:comment """StudyProgram which the course is part of.
"""@en;
    rdfs:isDefinedBy <http://linkedscience.org/teach/ns> .

teach:Teacher a owl:Class;
    rdfs:label "Teacher"@en;
    rdfs:comment """Teacher of the course.
"""@en;
    rdfs:isDefinedBy <http://linkedscience.org/teach/ns> .

teach: a prv:DataItem,
        owl:Ontology;
    dct:created "2013-04-25T18:09:00Z"^^xsd:dateTime;
    dct:creator <http://kauppinen.net/tomi#me>;
    dct:description """TEACH, the Teaching Core Vocabulary,
is a lightweight vocabulary providing terms to enable teachers to relate things in their courses together.
The Teaching Core Vocabulary is based on practical requirements set by providing seminar and course descriptions as Linked Data.
"""@en;
    dct:title "Teaching Core Vocabulary namespace"@en;
    prv:createdBy [ a prv:DataCreation;
            prv:performedAt "2013-04-25T18:09:00Z"^^xsd:dateTime;
            prv:performedBy <http://kauppinen.net/tomi#me> ] .

teach:academicTerm a owl:ObjectProperty;
    rdfs:label "academicTerm"@en;
    ns1:related <http://dbpedia.org/page/Academic_term>;
    rdfs:comment "academicTerm is an abstract property to express the academic term (e.g. Summer 2011) of the course/seminar."@en;
    rdfs:domain owl:thing;
    rdfs:isDefinedBy teach:academicTerm .

teach:arrangedAt a owl:ObjectProperty;
    rdfs:label "arrangedAt"@en;
    rdfs:comment """arrangedAt is an abstract property to explicate the date/time when the seminar is arranged at. It can be defined as in the following example:
  http://www.w3.org/TR/rdfcal/#L21805"""@en;
    rdfs:domain owl:thing;
    rdfs:isDefinedBy teach:arrangedAt;
    rdfs:range ical: .

teach:bookingNumber a owl:ObjectProperty;
    rdfs:label "bookingNumber"@en;
    ns1:related <http://dbpedia.org/page/Course_(education)>;
    rdfs:comment "bookingNumber is an abstract property to uniquely identify the course. This identifier should be defined and provided by the operator of the course."@en;
    rdfs:domain owl:thing;
    rdfs:isDefinedBy teach:bookingNumber;
    rdfs:subPropertyOf dct:description .

teach:building a owl:ObjectProperty;
    rdfs:label "room"@en;
    ns1:related <http://dbpedia.org/resource/Building>;
    rdfs:comment "building is an abstract property to express the building where the course/seminar takes place."@en;
    rdfs:domain owl:thing;
    rdfs:isDefinedBy teach:building .

teach:courseDescription a owl:ObjectProperty;
    rdfs:label "courseDescription"@en;
    ns1:related <http://dbpedia.org/page/Course_(education)>;
    rdfs:comment "courseDescription is subproperty of dc:description to specify the course description"@en;
    rdfs:domain owl:thing;
    rdfs:isDefinedBy teach:courseDescription;
    rdfs:subPropertyOf dct:description .

teach:courseTitle a owl:ObjectProperty;
    rdfs:label "courseTitle"@en;
    ns1:related <http://dbpedia.org/page/Course_(education)>;
    rdfs:comment "courseTitle is subproperty of dc:title to specify the course title"@en;
    rdfs:domain owl:thing;
    rdfs:isDefinedBy teach:courseTitle;
    rdfs:subPropertyOf dct:title .

teach:deadline a owl:ObjectProperty;
    rdfs:label "deadline"@en;
    rdfs:comment "deadline is an abstract property explicate the deadline for a draft project report."@en;
    rdfs:domain owl:thing;
    rdfs:isDefinedBy teach:deadline .

teach:deadlineDraftReport a owl:ObjectProperty;
    rdfs:label "deadlineDraftReport"@en;
    rdfs:comment "deadlineDraftReport is an abstract property explicate the deadline for a draft project report."@en;
    rdfs:domain owl:thing;
    rdfs:isDefinedBy teach:deadlineDraftReport .

teach:deadlineFinalReport a owl:ObjectProperty;
    rdfs:label "deadlineFinalReport"@en;
    rdfs:comment "deadlineFinalReport is an abstract property to explicate the deadline for a final project report."@en;
    rdfs:domain owl:thing;
    rdfs:isDefinedBy teach:deadlineFinalReport .

teach:deadlineReviewReport a owl:ObjectProperty;
    rdfs:label "deadlineReviewReport"@en;
    rdfs:comment "deadlineReviewReport is an abstract property to explicate the deadline for review reports (opponent works)."@en;
    rdfs:domain owl:thing;
    rdfs:isDefinedBy teach:deadlineReviewReport .

teach:ects a owl:ObjectProperty;
    rdfs:label "ects"@en;
    ns1:related <http://dbpedia.org/resource/European_Credit_Transfer_and_Accumulation_System>;
    rdfs:comment "ects is an abstract property to express the ects (European Credit Transfer System) of the course/seminar."@en;
    rdfs:domain owl:thing;
    rdfs:isDefinedBy teach:ects .

teach:grading a owl:ObjectProperty;
    rdfs:label "grading"@en;
    ns1:related <http://dbpedia.org/resource/Grading>;
    rdfs:comment "grading is an abstract property to relate the course/seminar to the description about its grading."@en;
    rdfs:domain owl:thing;
    rdfs:isDefinedBy teach:grading .

teach:hasDescription a owl:ObjectProperty;
    rdfs:label "hasDescription"@en;
    ns1:related <http://dbpedia.org/page/Course_(education)>;
    rdfs:comment "hasDescription is subproperty of dc:description to specify needed descriptions of entities within the course, e.g. the description of course materials, assignments, etc."@en;
    rdfs:isDefinedBy teach:hasDescription;
    rdfs:subPropertyOf dct:description .

teach:hasTeachingMethod a owl:ObjectProperty;
    rdfs:label "room"@en;
    rdfs:comment """Describes the teaching method used in the course/seminar. property "hasTeachingMethod" inspired by an interview of Nobel Laureate Carl Wieman in "Transformation Is Possible
If a University Really Cares", SCIENCE, Vol 340, April 19th, 2013: "Wieman came up with his simple, market-driven first step: Require universities to compile and release data on their teaching methods as a condition for receiving federal research funds. As students began using the data released by universities to help choose a college, he reasoned, universities would feel compelled to improve their teaching practices in order to attract the best applicants." The idea is that with the hasTeachingMethod-property universities can start publishing the teaching methods they use as Linked Open Data. Let us see which university implements the idea first."""@en;
    rdfs:domain owl:thing;
    rdfs:isDefinedBy teach:hasTeachingMethod .

teach:hasTitle a owl:ObjectProperty;
    rdfs:label "hasTitle"@en;
    ns1:related <http://dbpedia.org/page/Course_(education)>;
    rdfs:comment "hasTitle is subproperty of dc:title  to specify needed titles of entities within the course, e.g. the title of course materials, assignments, etc."@en;
    rdfs:isDefinedBy teach:hasTitle;
    rdfs:subPropertyOf dct:title .

teach:module a owl:ObjectProperty;
    rdfs:label "room"@en;
    ns1:related <http://dbpedia.org/resource/Module>;
    rdfs:comment "Describes the module of the study program with which the course/seminar is associated."@en;
    rdfs:domain owl:thing;
    rdfs:isDefinedBy teach:module .

teach:nextReading a owl:ObjectProperty;
    rdfs:label "nextReading"@en;
    rdfs:comment "nextReading is an abstract property for dynamically stating the reading required to be read by the next session of the course/seminar."@en;
    rdfs:domain owl:thing;
    rdfs:isDefinedBy teach:nextReading .

teach:notArrangedAt a owl:ObjectProperty;
    rdfs:label "notArrangedAt"@en;
    rdfs:comment "notArrangedAt is an abstract property to explicate the date/time when the seminar has an exception in its schedule and thus is not arranged at."@en;
    rdfs:domain owl:thing;
    rdfs:isDefinedBy teach:notArrangedAt;
    rdfs:range xsd:datetime .

teach:opponentOf a owl:ObjectProperty;
    rdfs:label "opponentOf"@en;
    rdfs:comment "opponentOf is an abstract property to state that a student is an opponent of another, i.e. that he/she makes review of the other student's seminar work."@en;
    rdfs:domain foaf:Agent;
    rdfs:isDefinedBy teach:opponentOf;
    rdfs:range foaf:Agent .

teach:reading a owl:ObjectProperty;
    rdfs:label "reading"@en;
    rdfs:comment "reading is an abstract property to relate required readings to the course/seminar."@en;
    rdfs:domain owl:thing;
    rdfs:isDefinedBy teach:reading .

teach:reportTemplate a owl:ObjectProperty;
    rdfs:label "reportTemplate"@en;
    rdfs:comment "reportTemplate is an abstract property to relate a report template to the course/seminar so that students may use it to write their reports."@en;
    rdfs:domain owl:thing;
    rdfs:isDefinedBy teach:reportTemplate .

teach:reviewTemplate a owl:ObjectProperty;
    rdfs:label "reviewTemplate"@en;
    rdfs:comment "reviewTemplate is an abstract property to relate a review template to the course/seminar so that students may use it to write their reviews of other student's reports."@en;
    rdfs:domain owl:thing;
    rdfs:isDefinedBy teach:reviewTemplate .

teach:room a owl:ObjectProperty;
    rdfs:label "room"@en;
    ns1:related <http://dbpedia.org/resource/Room>;
    rdfs:comment "room is an abstract property to express the room where the course/seminar takes place."@en;
    rdfs:domain owl:thing;
    rdfs:isDefinedBy teach:room .

teach:studentGroup a owl:ObjectProperty;
    rdfs:label "studentGroup"@en;
    ns1:related <http://dbpedia.org/resource/TEACHER>;
    rdfs:comment "studentGroup is an abstract property to relate a student group to the course/seminar."@en;
    rdfs:domain owl:thing;
    rdfs:isDefinedBy teach:studentGroup;
    rdfs:range foaf:Group .

teach:studyProgram a owl:ObjectProperty;
    rdfs:label "room"@en;
    rdfs:comment "Describes the study program which is associated with the course/seminar."@en;
    rdfs:domain owl:thing;
    rdfs:isDefinedBy teach:studyProgram .

teach:teacher a owl:ObjectProperty;
    rdfs:label "teacher"@en;
    ns1:related <http://dbpedia.org/resource/TEACHER>;
    rdfs:comment "teacher is an abstract property to relate a teacher to a course/seminar."@en;
    rdfs:domain owl:thing;
    rdfs:isDefinedBy teach:teacher;
    rdfs:range owl:thing .

teach:teacherOf a owl:ObjectProperty;
    rdfs:label "teacherOf"@en;
    ns1:related <http://dbpedia.org/resource/TEACHER>;
    rdfs:comment "teacherOf is an abstract property to relate a teacher to a course/seminar."@en;
    rdfs:domain owl:thing;
    rdfs:isDefinedBy teach:teacherOf;
    rdfs:range owl:thing .

teach:weeklyHours a owl:ObjectProperty;
    rdfs:label "weeklyHours"@en;
    ns1:related <http://de.dbpedia.org/resource/Semesterwochenstunde>;
    rdfs:comment "weeklyHours is an abstract property to express the number of weekly hours for the teaching."@en;
    rdfs:domain owl:thing;
    rdfs:isDefinedBy teach:weeklyHours .

<http://kauppinen.net/tomi#me> a foaf:Person;
    foaf:homepage <http://kauppinen.net/tomi>;
    foaf:name "Tomi Kauppinen"@en .

<http://linkedscience.org/teach/ns> a foaf:Document;
    rdfs:label "Document that defines the Teaching Core Vocabulary"@en;
    dct:conformsTo <http://www.w3.org/TR/rdfa-syntax>;
    dct:description "This documents specifies the classes and properties introduced by the TEACH core vocabulary."@en;
    dct:title "Teaching Core Vocabulary Specification"@en;
    xhv:license <http://creativecommons.org/licenses/by/1.0/>;
    foaf:primaryTopic teach: .

